src/Helpers/List.v
@@ -9,7 +9,15 @@ Section list.
   Notation list := (list A).
   Implicit Types l : list.
 
-  (* TODO: upstream. *)
+  Lemma list_filter_singleton (P : A → Prop)
+      `{!∀ x, Decision (P x)} x :
+    (filter P [x] = [] ∧ ¬ P x) ∨ (filter P [x] = [x] ∧ P x).
+  Proof.
+    destruct (decide $ P x).
+    - right. split; [|done]. rewrite filter_cons_True; [naive_solver|done].
+    - left. split; [|done]. rewrite filter_cons_False; [naive_solver|done].
+  Qed.
+
   Lemma list_filter_iff_strong (P1 P2 : A → Prop)
       `{!∀ x, Decision (P1 x), !∀ x, Decision (P2 x)} l :
     (∀ i x, l !! i = Some x → (P1 x ↔ P2 x)) →
@@ -23,7 +31,6 @@ Section list.
     - rewrite !filter_cons_False; [by naive_solver..|]. by rewrite IH.
   Qed.
 
-  (* TODO: upstream. *)
   Lemma list_filter_all (P : A → Prop)
       `{!∀ x, Decision (P x)} l :
     (∀ i x, l !! i = Some x → P x) →
@@ -35,10 +42,12 @@ Section list.
     rewrite filter_cons_True; [done|]. by rewrite IH.
   Qed.
 
-  (* TODO: upstream. *)
   Lemma lookup_snoc l x :
     (l ++ [x]) !! (length l) = Some x.
-  Proof. by opose proof (proj2 (lookup_snoc_Some _ _ (length l) x) _) as ?; [naive_solver|]. Qed.
+  Proof.
+    opose proof (proj2 (lookup_snoc_Some _ _ (length l) x) _) as ?;
+      [naive_solver|done].
+  Qed.
 
   Lemma list_singleton_exists l :
     length l = 1 →
